feat: Optimize sort by `Below`
The `Below` function is in the hot path.
The slice (x[1..]) operation is not optimized in Dafny.
This optimizes this function by turning the recursive slice
into a loop over an index into the seq.
Further, a bounded integer version is also included.

DynamoDbEncryption/dafny/StructuredEncryption/src/SortCanon.dfy
@@ -148,11 +148,89 @@ module SortCanon {
     }
   }
 
-  predicate method Below(x: seq<uint8>, y: seq<uint8>) {
+  predicate Below(x: seq<uint8>, y: seq<uint8>) {
     |x| != 0 ==>
       && |y| != 0
       && x[0] <= y[0]
       && (x[0] == y[0] ==> Below(x[1..], y[1..]))
+  } by method {
+
+    // The slice x[1..], y[1..] are un-optimized operations in Dafny.
+    // This means that their usage will result in a lot of data copying.
+    // Additional, it is very likely that these size of these sequences
+    // will be less than uint64.
+    // So writing an optimized version that only works on bounded types
+    // should further optimized this hot code.
+
+    if HasUint64Len(x) && HasUint64Len(y) {
+      return BoundedBelow(x,y);
+    }
+
+    if |x| == 0 {
+      assert Below(x, y);
+      return true;
+    }
+
+    if |y| == 0 {
+      assert !Below(x, y);
+      return false;
+    }
+
+    for i := 0 to |x|
+      invariant i <= |y|
+      // The function on the initial arguments
+      // is equal to function applied to the intermediate arguments.
+      invariant Below(x, y) == Below(x[i..], y[i..])
+    {
+      if |y| <= i {
+        return false;
+      } else if y[i] < x[i] {
+        return false;
+      } else if x[i] < y[i] {
+        return true;
+      } else {
+        assert x[i] == y[i];
+      }
+    }
+
+    return true;
+  }
+
+  predicate BoundedBelow(x: seq64<uint8>, y: seq64<uint8>)
+  {
+    Below(x,y)
+  } by method {
+    var xLength := |x| as uint64;
+    var yLength := |y| as uint64;
+
+    if xLength == 0 {
+      assert BoundedBelow(x, y);
+      return true;
+    }
+
+    if yLength == 0 {
+      assert !BoundedBelow(x, y);
+      return false;
+    }
+
+    for i := 0 to xLength
+      invariant i <= yLength
+      // The function on the initial arguments
+      // is equal to function applied to the intermediate arguments.
+      invariant BoundedBelow(x, y) == BoundedBelow(x[i..], y[i..])
+    {
+      if yLength <= i {
+        return false;
+      } else if y[i] < x[i] {
+        return false;
+      } else if x[i] < y[i] {
+        return true;
+      } else {
+        assert x[i] == y[i];
+      }
+    }
+
+    return true;
   }
 
   lemma BelowIsTotal()
